WIP on correctness, I have to find a way of using store_rule

Simu/Cor.v
@@ -4,7 +4,7 @@ Require Import cfrontend.Ctypes.
 Require Import lib.Integers.
 Require Import lib.Maps.
 Require Import lib.Coqlib.
-Require Import Errors.
+Require Errors.
 Require Import common.Separation.
 Require Import common.Values.
 Require Import common.Memory.
@@ -92,21 +92,21 @@ Section PRESERVATION.
       well_formed_exp c m (Const cst ty).
 
   Inductive well_formed_stmt (c: class) (m: method) (S: state): stmt -> Prop :=
-  | wf_assign: forall x e v,
+  | wf_assign: forall x e,
       In (x, typeof e) (meth_vars m) ->
       x <> self_id ->
       well_formed_exp c m e ->
-      exp_eval S e v ->
-      valid_val v (typeof e) ->
-      v = Values.Val.load_result (chunk_of_type (typeof e)) v ->
+      (* exp_eval S e v -> *)
+      (* valid_val v (typeof e) -> *)
+      (* v = Values.Val.load_result (chunk_of_type (typeof e)) v -> *)
       well_formed_stmt c m S (Assign x e)
-  | wf_assignst: forall x e v,
+  | wf_assignst: forall x e,
       In (x, typeof e) c.(c_mems) ->
       x <> self_id ->
       well_formed_exp c m e ->
-      exp_eval S e v ->
-      valid_val v (typeof e) ->
-      v = Values.Val.load_result (chunk_of_type (typeof e)) v ->
+      (* exp_eval S e v -> *)
+      (* valid_val v (typeof e) -> *)
+      (* v = Values.Val.load_result (chunk_of_type (typeof e)) v -> *)
       well_formed_stmt c m S (AssignSt x e)
   | wf_ite: forall e s1 s2,
       well_formed_exp c m e ->
@@ -182,9 +182,44 @@ Section PRESERVATION.
                            | None => False
                            end) (f.(m_in) ++ f.(m_vars))) ->
       match_states c f S (e, le, m).
-         
+
+  Lemma evall_out_field:
+    forall e le m f c x ty b d outco,
+      In (x, ty) f.(m_out) ->
+      le ! out_id = Some (Vptr b Int.zero) ->
+      field_offset tge x (co_members outco) = Errors.OK d ->
+      tge.(genv_cenv) ! (prefix f.(m_name) c.(c_name)) = Some outco ->
+        eval_lvalue tge e le m (deref_field out_id (prefix (m_name f) (c_name c)) x ty) b
+                    (Int.add Int.zero (Int.repr d)).
+  Proof.
+    intros.
+    apply* eval_Efield_struct.
+    + apply* eval_Elvalue.
+      apply* deref_loc_copy.
+    + simpl; unfold type_of_inst; eauto.
+  Qed.
+
+   Lemma eval_out_field:
+    forall S e le m f c x ty v outco outb,
+      In (x, ty) f.(m_out) ->
+      le ! out_id = Some (Vptr outb Int.zero) ->
+      tge.(genv_cenv) ! (prefix f.(m_name) c.(c_name)) = Some outco ->
+      In (x, ty) (co_members outco) ->
+      m |= blockrep tge S (co_members outco) outb ->
+      (* match_states c f S (e, le , m) -> *)
+      find_var S x v ->
+      eval_expr tge e le m (deref_field out_id (prefix (m_name f) (c_name c)) x ty) v.
+   Proof.
+     intros.
+     forwards* (? & Hoffset): blockrep_field_offset.
+     apply* eval_Elvalue.
+     - apply* evall_out_field.
+     - rewrite Int.add_zero_l.
+       apply* blockrep_deref_mem. 
+   Qed.
+   
   Lemma expr_eval_simu:
-    forall c S exp prog' clsnm  v e le m f,
+    forall c S exp prog' clsnm v e le m f,
       find_class clsnm prog = Some (c, prog') ->
       match_states c f S (e, le , m) ->
       well_formed_exp c f exp ->
@@ -208,14 +243,7 @@ Section PRESERVATION.
             (now apply in_or_app; right; apply in_or_app; right).
         app_NoDupMembers_det.
         forwards* (? & Hoffset): blockrep_field_offset.
-        eapply eval_Elvalue.
-        *{ apply* eval_Efield_struct.
-           - apply* eval_Elvalue.
-             apply* deref_loc_copy.
-           - simpl; unfold type_of_inst; eauto.
-         }
-        * rewrite Int.add_zero_l.
-          apply* blockrep_deref_mem. 
+        apply* eval_out_field.
       + apply sep_proj2, sep_proj2, sep_comm, sep_pure in Hrep.
         destruct Hrep as (Hrep & H); clear H.
         apply eval_Etempvar.
@@ -232,164 +260,398 @@ Section PRESERVATION.
           simpl in Hrep; destruct Hrep as (? & ? & ?).
           destruct (le ! x); [now app_match_find_var_det | contradiction].
 
-          
     (* State x ty : "self->x" *)
     - inverts WF.
       simpl.
-      forwards* (? & ? & ? & ? & ?): make_members_co.
-      apply find_class_name in Find; subst.
-      forwards* (? & Hoffset): staterep_field_offset. skip. skip.
-      eapply eval_Elvalue.
-      + apply* eval_Efield_struct.
-        *{ apply* eval_Elvalue.
-           apply* deref_loc_copy.
-         } 
-        * simpl; unfold type_of_inst; eauto.
-        * skip.
-      + eapply deref_loc_value.
-        * simpl. skip.
-        * skip.
-        
+      apply sep_proj1 in Hrep.
+      forwards* (? & Hco & ? & Eq & ? & Nodup): make_members_co; instantiate (1:=tprog) in Hco.
+      forwards ?: find_class_name Find; subst.
+      forwards (? & Hprog & FindNone): find_class_app Find.
+      rewrite Hprog in Hrep.
+      rewrite staterep_skip_app in Hrep.
+      assert (In (i, t) (make_members c)) by
+          (unfold make_members; rewrite in_app_iff; now left).
+      + forwards* (? & Hoffset): staterep_field_offset. 
+        eapply eval_Elvalue.
+        *{ apply* eval_Efield_struct.
+           - apply* eval_Elvalue.
+             apply* deref_loc_copy. 
+           - simpl; unfold type_of_inst; eauto.
+           - rewrite* Eq. 
+         }
+        * apply* staterep_deref_mem.
+          (* rewrite Int.unsigned_repr_eq. *)
+          rewrite* Int.unsigned_repr.
+          rewrite Eq in Nodup.
+          forwards* Ftype: field_translate_mem_type.
+          eapply field_offset_in_range in Hoffset; eauto.
+          split*.
+          admit.
+      + intro Hin.
+        apply ClassIn_find_class in Hin.
+        contradiction.
+
     (* Const c ty : "c" *)
     - destruct cst; constructor.
-  Admitted.
+  Qed.
+
+  Lemma exp_eval_valid:
+    forall S e v,
+      exp_eval S e v -> valid_val v (typeof e).
+  Proof.
+    induction 1; auto.
+  Qed.
+
+  Lemma exp_eval_access:
+    forall S e v,
+      exp_eval S e v -> access_mode (typeof e) = By_value (chunk_of_type (typeof e)).
+  Proof.
+    introv H.
+    apply exp_eval_valid in H.
+    apply* valid_val_access.
+  Qed.
+
+  Hint Resolve exp_eval_valid exp_eval_access.
 
   Lemma exprs_eval_simu:
-    forall c S es es' vs e le m,
-      compat_vars c S e m ->
-      compat_self c S e m ->
-      In c prog ->
-      Nelist.Forall (well_formed_exp c) es ->
-      Nelist.Forall2 (fun e v => valid_val v (typeof e)) es vs ->
-      Nelist.Forall2 (exp_eval S) es vs ->
-      es' = nelist2list (Nelist.map (translate_exp c.(c_name)) es) ->
-      Clight.eval_exprlist tge e le m es' (list_type_to_typelist (map Clight.typeof es')) (nelist2list vs).
+    forall c S es es' prog' clsnm vs e le m f,
+      find_class clsnm prog = Some (c, prog') ->
+      match_states c f S (e, le , m) ->
+      Forall (well_formed_exp c f) es ->
+      Forall2 (exp_eval S) es vs ->
+      es' = map (translate_exp c f) es ->
+      Clight.eval_exprlist tge e le m es'
+                           (list_type_to_typelist (map Clight.typeof es')) vs.
   Proof.
     Hint Constructors Clight.eval_exprlist.
-    introv ? ? ? Hwf Hvalid Hev ?; subst es';
-    induction Hev; inverts Hwf; inverts Hvalid; econstructor;
+    introv Find MS WF EV ?; subst es';
+      induction EV; inverts WF; econstructor;
     (apply* expr_eval_simu || (rewrite type_pres; apply* sem_cast_same) || eauto).
   Qed.
 
   Remark eval_exprlist_app:
     forall e le m es es' vs vs',
-      Clight.eval_exprlist tge e le m es (list_type_to_typelist (map Clight.typeof es)) vs ->
-      Clight.eval_exprlist tge e le m es' (list_type_to_typelist (map Clight.typeof es')) vs' ->
-      Clight.eval_exprlist tge e le m (es ++ es') (list_type_to_typelist (map Clight.typeof (es ++ es'))) (vs ++ vs').
+      Clight.eval_exprlist tge e le m es
+                           (list_type_to_typelist (map Clight.typeof es)) vs ->
+      Clight.eval_exprlist tge e le m es'
+                           (list_type_to_typelist (map Clight.typeof es')) vs' ->
+      Clight.eval_exprlist tge e le m (es ++ es')
+                           (list_type_to_typelist (map Clight.typeof (es ++ es'))) (vs ++ vs').
   Proof.
     induction es; introv Ev Ev'; inverts* Ev.
     repeat rewrite <-app_comm_cons.
     simpl; econstructor; eauto.
   Qed.
+
+  (*   forall c S e m loc x t v, *)
+  (*     In c prog -> *)
+  (*     match_states c S (e, m) -> *)
+  (*     Maps.PTree.get x e = Some (loc, t) -> *)
+  (*     In (x, t) (class_vars c) -> *)
+  (*     v = Values.Val.load_result (chunk_of_type t) v -> *)
+  (*     valid_val v t -> *)
+  (*     x <> self_id -> *)
+  (*     exists m', Memory.Mem.store (chunk_of_type t) m loc 0 v = Some m'  *)
+  (*           /\ match_states c (update_var S x v) (e, m'). *)
+  (* Lemma match_states_assign_out: *)
+  (*     forall c f S e le m, *)
+  (*       match_states c f S (e, le, m) -> *)
+  (*       In (x, t) f.(m_out) -> *)
+  (*       exists m', Memory.Mem.store (chunk_of_type t) m loc 0 v = Some m' *)
+  (*             /\ match_states c (update_var S x v) (e, m'). *)
+    
+  (* Hint Constructors Clight.eval_lvalue Clight.eval_expr well_formed_stmt. *)
+  Hint Resolve expr_eval_simu Clight.assign_loc_value exp_eval_valid sem_cast_same.
   
-  Definition nodup_env (e: Clight.env) :=
-    forall x x' loc t t',
-      x' <> x ->
-      Maps.PTree.get x e = Some (loc, t) ->
-      Maps.PTree.get x' e <> Some (loc, t').
+  Theorem correctness:
+    forall c prog' f s S1 S2,
+      stmt_eval prog S1 s S2 ->
+      find_class c.(c_name) prog = Some (c, prog') ->
+      well_formed_stmt c f S1 s ->
+      forall e1 le1 m1,
+        match_states c f S1 (e1, le1, m1) ->
+        exists le2 m2 t,
+          exec_stmt tge (function_entry2 tge) e1 le1 m1
+                    (translate_stmt prog c f s) t le2 m2 Out_normal
+          /\ match_states c f S2 (e1, le2, m2).
+  Proof.
+    remember prog.
+    clear TRANSL main_node_exists.
+    introv EV; induction EV; introv Find WF MS; subst; inverts WF;
+    pose proof MS as MS'; inverts MS' as Hself Hout Houtco Hflds Hrep.
 
-  Definition nodup_fields (co: Ctypes.composite) :=
-    forall x t t',
-      In (x, t) (Ctypes.co_members co) ->
-      In (x, t') (Ctypes.co_members co) ->
-      t' = t.
+    (* Assign x e : "x = e" *)
+    - (* app_exp_eval_det. *)
+      simpl; unfold assign.
+      destruct (existsb (fun out => ident_eqb (fst out) x) f.(m_out)) eqn: E.
+      + do 3 econstructor; split.
+        *{ apply sep_pick2 in Hrep.
+           apply existsb_exists in E.
+           destruct E as ((x' & ty') & Hin & E).
+           rewrite ident_eqb_eq in E; simpl in E; subst. 
+           pose proof (m_nodup f) as Nodup.
+           assert (In (x, ty') (meth_vars f)) by
+               (now apply in_or_app; right; apply in_or_app; right).
+           app_NoDupMembers_det.
+           forwards* (? & Hoffset): blockrep_field_offset.
+           apply* ClightBigstep.exec_Sassign.
+           - apply* evall_out_field. 
+           - rewrite* type_pres; apply* sem_cast_same; apply* exp_eval_valid.
+           - apply* assign_loc_value.
+             + simpl. apply* exp_eval_access.
+             + skip. 
+        * skip.
+      + do 3 econstructor; split.
+        apply* ClightBigstep.exec_Sset.
+        admit.
+      
+    (* AssignSt x e : "self->x = e"*)
+    - app_exp_eval_det.
+      do 3 econstructor; split*.
+      + apply* ClightBigstep.exec_Sassign.
+        skip.
+        rewrite* type_pres.
+        skip.
+      + skip.
+      
+    (* Ifte e s1 s2 : "if e then s1 else s2" *)
+    - edestruct IHEV; destruct_conjs; eauto; [destruct*b|]. 
+      do 3 econstructor; split*.
+      apply* exec_Sifthenelse.
+      + erewrite type_pres, bool_val_ptr; eauto.
+      + destruct* b.
+      
+    (* Comp s1 s2 : "s1; s2" *)
+    - app_stmt_eval_det.
+      edestruct IHEV1; destruct_conjs; eauto.
+      edestruct IHEV2; destruct_conjs; eauto.
+      do 3 econstructor; split*.
+      apply* exec_Sseq_1.
+      
+    (* Step_ap y ty clsid o [e1; ... ;en] : "y = clsid_step(&(self->o), e1, ..., en)" *)
+    - (* app_exps_eval_det. *)
+      (* app_find_inst_det. *)
+      (* app_stmt_step_eval_det'. *)
+      
+      (* (* get the Clight corresponding function *) *)
+      (* forwards* Hin': find_class_In Hfind. *)
+      (* pose proof Hstep as Hstep'. *)
+      (* edestruct Hstep' as (loc_f & f & ? & ? & ? & Htype_fun & ? & ? & Hlengths & ?); eauto. *)
+      (* rewrite <-type_pres' with (c:=c) (es:=es) (ys:=ys) in Htype_fun; auto. *)
+      (* forwards Eq: find_class_name Hfind. *)
+      (* rewrite Eq in *; clear Eq. *)
+      
+      (* (* get the Clight corresponding field *) *)
+      (* pose proof Hself as Hself'. *)
+      (* destruct* Hself' as (? & ? & ? & ? & ? & ? & ? & ? & Hobj). *)
+      (* specializes Hobj Hin; destruct Hobj.  *)
 
-  Definition nodup_vars (c: class) :=
-    forall x t t',
-      In (x, t) (class_vars c) ->
-      In (x, t') (class_vars c) ->
-      t' = t.
+      (* (* get outs values *) *)
+      (* edestruct exprlist_make_out_arg with (le:=le1) (c:=c) as (outs); eauto. *)
+      
+      (* (* recursive funcall evaluation *) *)
+      (* edestruct Hrec_eval with (c:=c) (e:=e1) (m:=m1) (le:=le1) (outs:=outs); destruct_conjs; eauto. *)
+      (* + rewrite <-ne_Forall2_lengths with (1:=Evs). *)
+      (*   rewrite Hlengths; simpl; f_equal. *)
+      (*   rewrite app_length; do 2 rewrite <-nelist2list_length. *)
+      (*   f_equal; symmetry; apply* ne_Forall2_lengths.         *)
+      (* + apply Clight.eval_Eaddrof; apply* evall_self_field. *)
+      (* + do 3 econstructor; split*. *)
+      (*   *{ apply* exec_Scall. *)
+      (*      - simpl; eauto. *)
+      (*      - eapply Clight.eval_Elvalue. *)
+      (*        + apply* Clight.eval_Evar_global. *)
+      (*        + apply* Clight.deref_loc_reference. *)
+      (*      - econstructor. *)
+      (*        + eapply Clight.eval_Eaddrof. *)
+      (*          apply* evall_self_field. *)
+      (*        + eapply sem_cast_same. *)
+      (*          unfold valid_val; splits*. *)
+      (*          * discriminate. *)
+      (*          * simpl; trivial. *)
+      (*        + apply* eval_exprlist_app. *)
+      (*          apply* exprs_eval_simu. *)
+      (*      - eauto. *)
+      (*    } *)
+      (*   * admit.  *)
+      admit.
+      
+    (* Skip : "skip" *)
+    - do 3 econstructor; split*.
+      eapply exec_Sskip.
 
-   Definition nodup_mems (c: class) :=
-    forall x t t',
-      In (x, t) c.(c_mems) ->
-      In (x, t') c.(c_mems) ->
-      t' = t.
+    (* funcall *)
+    (* - (* forwards* Hfind'': find_class_sub_same Hfind UNIQUE. *) *)
+      (* rewrite Hfind' in Hfind''; inverts Hfind''. *)
+      (* destruct Hstep with (c:=cls) *)
+      (*   as (loc_f' & f' & Hget_loc_f' & Hget_f' & Htype_fun & Hvars_nil & ? & ? & Htr & ?); *)
+      (*   destruct_conjs; eauto. *)
+      (* forwards Eq: find_class_name Hfind. *)
+      (* rewrite Eq in Hget_loc_f'; clear Eq. *)
+      (* rewrite Hget_loc_f' in Hget_loc_f; inverts Hget_loc_f. *)
+      (* rewrite Hget_f' in Hget_f; inverts Hget_f. *)
+
+      (* assert (length f.(Clight.fn_params) = length ((Values.Vptr loc_struct ofs) :: nelist2list vs)) *)
+      (*   by (rewrite Hlengths; simpl; f_equal; rewrite Nelist.nelist2list_length; auto). *)
+
+      (* forwards* (le_fun & ? & ?): (compat_funcall_pres cls m). *)
+      (* forwards* Hsub: find_class_sub. *)
+      (* subst env. *)
+      (* edestruct Hrec_exec with (le1:=le_fun) as (? & ? & ? & ? & MS); eauto. *)
+      (* destruct_conjs. *)
+        
+      (* do 2 econstructor; split. *)
+      (* apply* eval_funcall_internal. *)
+      (* + constructor*; rewrite Hvars_nil; simpl; constructor. *)
+      (* + rewrite* Htr. *)
+      (*   apply* exec_Sseq_1. *)
+      (*   apply* exec_Sreturn_some. *)
+      (*   apply* Clight.eval_Etempvar. *)
+      (*   inverts MS as Hvars'. *)
+      (*   apply* Hvars'; rewrite <-surjective_pairing; eapply in_eq. *)
+      (* + simpl; split*. *)
+      (*   inverts Htype_fun. *)
+      (*   apply* sem_cast_same. *)
+      (* + simpl; eauto.        *)
+      (* + constructor*. *)
+      (*   unfold compat_self. *)
+      (*   intro Hin. *)
+      (*   pose proof Hself as Hself'. *)
+      (*   destruct* Hself' as (? & loc_struct' & ofs' & Hget_self' & Hget_co' & Hmem & Hobj). *)
+      (*   do 3 econstructor; splits*. *)
+      (*   intros x' t' Hin'.  *)
+      (*   specializes Hmem Hin'; destruct Hmem. *)
+      (*   econstructor; splits*. *)
+      (*   * admit. *)
+      (*   * admit. *)
+  Qed.
   
-  Remark find_add:
-    forall x (v v': val) pm, 
-      PM.find x (PM.add x v pm) = Some v' -> v' = v.
-  Proof.
-    induction x, pm; simpl; (eauto || now injection 1).
-  Qed.
+  
+  (* Definition nodup_env (e: Clight.env) := *)
+  (*   forall x x' loc t t', *)
+  (*     x' <> x -> *)
+  (*     Maps.PTree.get x e = Some (loc, t) -> *)
+  (*     Maps.PTree.get x' e <> Some (loc, t'). *)
 
-  Remark find_update_var:
-    forall x v v' S,
-      find_var (update_var S x v) x v' -> v' = v.
-  Proof.
-    unfold find_var, update_var; simpl.
-    intros; apply* find_add.
-  Qed.
+  (* Definition nodup_fields (co: Ctypes.composite) := *)
+  (*   forall x t t', *)
+  (*     In (x, t) (Ctypes.co_members co) -> *)
+  (*     In (x, t') (Ctypes.co_members co) -> *)
+  (*     t' = t. *)
 
-  Remark find_update_field:
-    forall x v v' S,
-      find_field (update_field S x v) x v' -> v' = v.
-  Proof.
-    unfold find_field, update_field, mfind_mem, madd_mem; simpl.
-    intros; apply* find_add.
-  Qed.
+  (* Definition nodup_vars (c: class) := *)
+  (*   forall x t t', *)
+  (*     In (x, t) (class_vars c) -> *)
+  (*     In (x, t') (class_vars c) -> *)
+  (*     t' = t. *)
 
-  Remark gso_var:
-    forall x x' v v' S,
-      x <> x' -> find_var (update_var S x' v) x v' -> find_var S x v'.
-  Proof.
-    unfold find_var, update_var; simpl.
-    introv Neq H.
-    rewrite <-H; symmetry.
-    apply* PM.gso.
-  Qed.
+  (*  Definition nodup_mems (c: class) := *)
+  (*   forall x t t', *)
+  (*     In (x, t) c.(c_mems) -> *)
+  (*     In (x, t') c.(c_mems) -> *)
+  (*     t' = t. *)
+  
+  (* Remark find_add: *)
+  (*   forall x (v v': val) pm,  *)
+  (*     PM.find x (PM.add x v pm) = Some v' -> v' = v. *)
+  (* Proof. *)
+  (*   induction x, pm; simpl; (eauto || now injection 1). *)
+  (* Qed. *)
 
-  Remark gso_field:
-    forall x x' v v' S,
-      x <> x' -> find_field (update_field S x' v) x v' -> find_field S x v'.
-  Proof.
-    unfold find_field, update_field; simpl.
-    introv Neq H.
-    rewrite <-H; symmetry.
-    apply* mfind_mem_gso.
-  Qed.
+  (* Remark find_update_var: *)
+  (*   forall x v v' S, *)
+  (*     find_var (update_var S x v) x v' -> v' = v. *)
+  (* Proof. *)
+  (*   unfold find_var, update_var; simpl. *)
+  (*   intros; apply* find_add. *)
+  (* Qed. *)
 
-  Remark find_field_update_var:
-    forall S x v x' v',
-      find_field (update_var S x v) x' v' -> find_field S x' v'.
-  Proof. unfold find_field, update_var; simpl; auto. Qed.
+  (* Remark find_update_field: *)
+  (*   forall x v v' S, *)
+  (*     find_field (update_field S x v) x v' -> v' = v. *)
+  (* Proof. *)
+  (*   unfold find_field, update_field, mfind_mem, madd_mem; simpl. *)
+  (*   intros; apply* find_add. *)
+  (* Qed. *)
 
-  Remark find_var_update_field:
-    forall S x v x' v',
-      find_var (update_field S x v) x' v' -> find_var S x' v'.
-  Proof. unfold find_var, update_field; simpl; auto. Qed.
+  (* Remark gso_var: *)
+  (*   forall x x' v v' S, *)
+  (*     x <> x' -> find_var (update_var S x' v) x v' -> find_var S x v'. *)
+  (* Proof. *)
+  (*   unfold find_var, update_var; simpl. *)
+  (*   introv Neq H. *)
+  (*   rewrite <-H; symmetry. *)
+  (*   apply* PM.gso. *)
+  (* Qed. *)
 
-  Definition mem_sep (c: class) (e: Clight.env) (m: Memory.Mem.mem) :=
-    forall x loc t loc_self loc_struct ofs,
-      In (x, t) (class_vars c) -> 
-      Maps.PTree.get x e = Some (loc, t) ->
-      Maps.PTree.get self_id e = Some (loc_self, pointer_of_node c.(c_name)) ->
-      Memory.Mem.load AST.Mint32 m loc_self 0 = Some (Values.Vptr loc_struct ofs) ->
-      loc <> loc_struct.
+  (* Remark gso_field: *)
+  (*   forall x x' v v' S, *)
+  (*     x <> x' -> find_field (update_field S x' v) x v' -> find_field S x v'. *)
+  (* Proof. *)
+  (*   unfold find_field, update_field; simpl. *)
+  (*   introv Neq H. *)
+  (*   rewrite <-H; symmetry. *)
+  (*   apply* mfind_mem_gso. *)
+  (* Qed. *)
 
-  Definition self_sep (c: class) (e: Clight.env) (m: Memory.Mem.mem) :=
-    forall loc_self loc_struct ofs,
-      Maps.PTree.get self_id e = Some (loc_self, pointer_of_node c.(c_name)) ->
-      Memory.Mem.load AST.Mint32 m loc_self 0 = Some (Values.Vptr loc_struct ofs) ->
-      loc_struct <> loc_self.
+  (* Remark find_field_update_var: *)
+  (*   forall S x v x' v', *)
+  (*     find_field (update_var S x v) x' v' -> find_field S x' v'. *)
+  (* Proof. unfold find_field, update_var; simpl; auto. Qed. *)
 
-  Definition fields_sep (m: Memory.Mem.mem) :=
-    forall co x x' t t' ofs delta delta',
-      x <> x' ->
-      Ctypes.field_offset (Clight.genv_cenv tge) x (Ctypes.co_members co) = Errors.OK delta ->
-      Ctypes.field_offset (Clight.genv_cenv tge) x' (Ctypes.co_members co) = Errors.OK delta' ->
-      (BinInt.Z.le
-         (BinInt.Z.add (Int.unsigned (Int.add ofs (Int.repr delta')))
-                       (Memdata.size_chunk (chunk_of_type t')))
-         (Int.unsigned (Int.add ofs (Int.repr delta)))
-       \/
-       BinInt.Z.le
-         (BinInt.Z.add (Int.unsigned (Int.add ofs (Int.repr delta)))
-                       (Memdata.size_chunk (chunk_of_type t)))
-         (Int.unsigned (Int.add ofs (Int.repr delta')))).
+  (* Remark find_var_update_field: *)
+  (*   forall S x v x' v', *)
+  (*     find_var (update_field S x v) x' v' -> find_var S x' v'. *)
+  (* Proof. unfold find_var, update_field; simpl; auto. Qed. *)
 
-  (* Hypothesis STEPS: *)
-  (*   forall c (e: Clight.env), *)
+  (* Definition mem_sep (c: class) (e: Clight.env) (m: Memory.Mem.mem) := *)
+  (*   forall x loc t loc_self loc_struct ofs, *)
+  (*     In (x, t) (class_vars c) ->  *)
+  (*     Maps.PTree.get x e = Some (loc, t) -> *)
+  (*     Maps.PTree.get self_id e = Some (loc_self, pointer_of_node c.(c_name)) -> *)
+  (*     Memory.Mem.load AST.Mint32 m loc_self 0 = Some (Values.Vptr loc_struct ofs) -> *)
+  (*     loc <> loc_struct. *)
+
+  (* Definition self_sep (c: class) (e: Clight.env) (m: Memory.Mem.mem) := *)
+  (*   forall loc_self loc_struct ofs, *)
+  (*     Maps.PTree.get self_id e = Some (loc_self, pointer_of_node c.(c_name)) -> *)
+  (*     Memory.Mem.load AST.Mint32 m loc_self 0 = Some (Values.Vptr loc_struct ofs) -> *)
+  (*     loc_struct <> loc_self. *)
+
+  (* Definition fields_sep (m: Memory.Mem.mem) := *)
+  (*   forall co x x' t t' ofs delta delta', *)
+  (*     x <> x' -> *)
+  (*     Ctypes.field_offset (Clight.genv_cenv tge) x (Ctypes.co_members co) = Errors.OK delta -> *)
+  (*     Ctypes.field_offset (Clight.genv_cenv tge) x' (Ctypes.co_members co) = Errors.OK delta' -> *)
+  (*     (BinInt.Z.le *)
+  (*        (BinInt.Z.add (Int.unsigned (Int.add ofs (Int.repr delta'))) *)
+  (*                      (Memdata.size_chunk (chunk_of_type t'))) *)
+  (*        (Int.unsigned (Int.add ofs (Int.repr delta))) *)
+  (*      \/ *)
+  (*      BinInt.Z.le *)
+  (*        (BinInt.Z.add (Int.unsigned (Int.add ofs (Int.repr delta))) *)
+  (*                      (Memdata.size_chunk (chunk_of_type t))) *)
+  (*        (Int.unsigned (Int.add ofs (Int.repr delta')))). *)
+
+  (* (* Hypothesis STEPS: *) *)
+  (* (*   forall c (e: Clight.env), *) *)
+  (* (*     In c prog -> *) *)
+  (* (*     exists loc_f f, *) *)
+  (* (*       Globalenvs.Genv.find_symbol tge.(Clight.genv_genv) (step_id c.(c_name)) = Some loc_f *) *)
+  (* (*       /\ Maps.PTree.get (step_id c.(c_name)) e = None *) *)
+  (* (*       /\ Globalenvs.Genv.find_funct_ptr tge.(Clight.genv_genv) loc_f = Some (Ctypes.Internal f) *) *)
+  (* (*       /\ Clight.type_of_fundef (Ctypes.Internal f) = *) *)
+  (* (*         Ctypes.Tfunction (Ctypes.Tcons (type_of_inst_p c.(c_name)) *) *)
+  (* (*                                        (list_type_to_typelist (map snd (nelist2list c.(c_input) ++ nelist2list c.(c_output))))) *) *)
+  (* (*                                        Ctypes.Tvoid AST.cc_default *) *)
+  (* (*       /\ Coqlib.list_norepet (Clight.var_names (Clight.fn_params f) ++ Clight.var_names (Clight.fn_vars f)) *) *)
+  (* (*       /\ Clight.fn_body f = snd (translate_stmt c.(c_name) c.(c_step)) *) *)
+  (* (*       /\ length f.(Clight.fn_params) = 1 + Nelist.length c.(c_input)   *) *)
+  (* (*       /\ Forall (fun x => Ctypes.access_mode (snd x) = Ctypes.By_value (chunk_of_type (snd x))) *) *)
+  (* (*                (f.(Clight.fn_params) ++ f.(Clight.fn_vars)). *) *)
+  
+  (* Definition match_step (e: Clight.env) := *)
+  (*   forall c, *)
   (*     In c prog -> *)
   (*     exists loc_f f, *)
   (*       Globalenvs.Genv.find_symbol tge.(Clight.genv_genv) (step_id c.(c_name)) = Some loc_f *)
@@ -397,162 +659,71 @@ Section PRESERVATION.
   (*       /\ Globalenvs.Genv.find_funct_ptr tge.(Clight.genv_genv) loc_f = Some (Ctypes.Internal f) *)
   (*       /\ Clight.type_of_fundef (Ctypes.Internal f) = *)
   (*         Ctypes.Tfunction (Ctypes.Tcons (type_of_inst_p c.(c_name)) *)
-  (*                                        (list_type_to_typelist (map snd (nelist2list c.(c_input) ++ nelist2list c.(c_output))))) *)
-  (*                                        Ctypes.Tvoid AST.cc_default *)
+  (*                                        (list_type_to_typelist *)
+  (*                                           (map snd (nelist2list c.(c_input) ++ nelist2list c.(c_output))))) *)
+  (*                          Ctypes.Tvoid AST.cc_default *)
+  (*       (* /\ f.(Clight.fn_vars) = [] *) *)
   (*       /\ Coqlib.list_norepet (Clight.var_names (Clight.fn_params f) ++ Clight.var_names (Clight.fn_vars f)) *)
-  (*       /\ Clight.fn_body f = snd (translate_stmt c.(c_name) c.(c_step)) *)
-  (*       /\ length f.(Clight.fn_params) = 1 + Nelist.length c.(c_input)   *)
+  (*       /\ Clight.fn_body f = Clight.Ssequence (translate_stmt c.(c_name) c.(c_step)) (Clight.Sreturn None) *)
+  (*       /\ f.(Clight.fn_params) = *)
+  (*         (self_id, type_of_inst_p c.(c_name)) :: nelist2list c.(c_input) ++ nelist2list c.(c_output) *)
   (*       /\ Forall (fun x => Ctypes.access_mode (snd x) = Ctypes.By_value (chunk_of_type (snd x))) *)
   (*                (f.(Clight.fn_params) ++ f.(Clight.fn_vars)). *)
   
-  Definition match_step (e: Clight.env) :=
-    forall c,
-      In c prog ->
-      exists loc_f f,
-        Globalenvs.Genv.find_symbol tge.(Clight.genv_genv) (step_id c.(c_name)) = Some loc_f
-        /\ Maps.PTree.get (step_id c.(c_name)) e = None
-        /\ Globalenvs.Genv.find_funct_ptr tge.(Clight.genv_genv) loc_f = Some (Ctypes.Internal f)
-        /\ Clight.type_of_fundef (Ctypes.Internal f) =
-          Ctypes.Tfunction (Ctypes.Tcons (type_of_inst_p c.(c_name))
-                                         (list_type_to_typelist
-                                            (map snd (nelist2list c.(c_input) ++ nelist2list c.(c_output)))))
-                           Ctypes.Tvoid AST.cc_default
-        (* /\ f.(Clight.fn_vars) = [] *)
-        /\ Coqlib.list_norepet (Clight.var_names (Clight.fn_params f) ++ Clight.var_names (Clight.fn_vars f))
-        /\ Clight.fn_body f = Clight.Ssequence (translate_stmt c.(c_name) c.(c_step)) (Clight.Sreturn None)
-        /\ f.(Clight.fn_params) =
-          (self_id, type_of_inst_p c.(c_name)) :: nelist2list c.(c_input) ++ nelist2list c.(c_output)
-        /\ Forall (fun x => Ctypes.access_mode (snd x) = Ctypes.By_value (chunk_of_type (snd x)))
-                 (f.(Clight.fn_params) ++ f.(Clight.fn_vars)).
-  
-  Definition c_state := (Clight.env * Memory.Mem.mem)%type.
+  (* Definition c_state := (Clight.env * Memory.Mem.mem)%type. *)
    
-  Inductive match_states (c: class) (S: state): c_state -> Prop :=
-    intro_match_states: forall e m,
-      (* state correspondance *)
-      compat_vars c S e m ->
-      compat_self c S e m ->
+  (* Inductive match_states (c: class) (S: state): c_state -> Prop := *)
+  (*   intro_match_states: forall e m, *)
+  (*     (* state correspondance *) *)
+  (*     compat_vars c S e m -> *)
+  (*     compat_self c S e m -> *)
 
-      (* function *)
-      match_step e ->
+  (*     (* function *) *)
+  (*     match_step e -> *)
       
-      (* Clight side separation *)
-      mem_sep c e m ->
-      self_sep c e m ->
-      fields_sep m ->
-      nodup_env e ->
+  (*     (* Clight side separation *) *)
+  (*     mem_sep c e m -> *)
+  (*     self_sep c e m -> *)
+  (*     fields_sep m -> *)
+  (*     nodup_env e -> *)
 
-      (* Minimp side separation *)
-      nodup_vars c ->
-      nodup_mems c ->
-      match_states c S (e, m).
+  (*     (* Minimp side separation *) *)
+  (*     nodup_vars c -> *)
+  (*     nodup_mems c -> *)
+  (*     match_states c S (e, m). *)
 
-  Hint Constructors match_states.
+  (* Hint Constructors match_states. *)
   
-  Remark load_same:
-    forall env x t x' t' m m' chk loc loc' v vptr vptr',
-      nodup_env env ->
-      x <> x' ->
-      Maps.PTree.get x env = Some (loc, t) ->
-      Maps.PTree.get x' env = Some (loc', t') ->
-      Memory.Mem.store chk m loc 0 v = Some m' ->
-      Memory.Mem.load AST.Mint32 m loc' 0 = Some vptr ->
-      Memory.Mem.load AST.Mint32 m' loc' 0 = Some vptr' ->
-      vptr' = vptr.
-  Proof.
-    introv Hnodupenv ? ? ? ? Hload Hload'.
-    destruct (Values.eq_block loc loc').
-      + subst loc.
-        edestruct Hnodupenv; eauto.
-      + assert (Memory.Mem.load AST.Mint32 m' loc' 0 = Memory.Mem.load AST.Mint32 m loc' 0)
-          as Eq by apply* Memory.Mem.load_store_other.
-        rewrite Eq in Hload'; rewrite Hload' in Hload; inverts Hload.
-        reflexivity.        
-  Qed.
+  (* Remark load_same: *)
+  (*   forall env x t x' t' m m' chk loc loc' v vptr vptr', *)
+  (*     nodup_env env -> *)
+  (*     x <> x' -> *)
+  (*     Maps.PTree.get x env = Some (loc, t) -> *)
+  (*     Maps.PTree.get x' env = Some (loc', t') -> *)
+  (*     Memory.Mem.store chk m loc 0 v = Some m' -> *)
+  (*     Memory.Mem.load AST.Mint32 m loc' 0 = Some vptr -> *)
+  (*     Memory.Mem.load AST.Mint32 m' loc' 0 = Some vptr' -> *)
+  (*     vptr' = vptr. *)
+  (* Proof. *)
+  (*   introv Hnodupenv ? ? ? ? Hload Hload'. *)
+  (*   destruct (Values.eq_block loc loc'). *)
+  (*     + subst loc. *)
+  (*       edestruct Hnodupenv; eauto. *)
+  (*     + assert (Memory.Mem.load AST.Mint32 m' loc' 0 = Memory.Mem.load AST.Mint32 m loc' 0) *)
+  (*         as Eq by apply* Memory.Mem.load_store_other. *)
+  (*       rewrite Eq in Hload'; rewrite Hload' in Hload; inverts Hload. *)
+  (*       reflexivity.         *)
+  (* Qed. *)
   
-  Lemma compat_assign_pres:
-    forall c S e m loc x t v,
-      In c prog ->
-      match_states c S (e, m) ->
-      Maps.PTree.get x e = Some (loc, t) ->
-      In (x, t) (class_vars c) ->
-      v = Values.Val.load_result (chunk_of_type t) v ->
-      valid_val v t ->
-      x <> self_id ->
-      exists m', Memory.Mem.store (chunk_of_type t) m loc 0 v = Some m' 
-            /\ match_states c (update_var S x v) (e, m').
-  Proof.
-    introv ? MS Hget Hin Hloadres ? ?.
-    inverts MS as Hvars Hself Hstep Hsep Hself_sep Hfields_sep Hnodupenv Hnodupvars; intro Hnodupmems.
-    edestruct Hvars as (loc' & Hget' & ? & ?); eauto.
-    rewrite Hget' in Hget; inverts Hget; rename Hget' into Hget.
-    edestruct Memory.Mem.valid_access_store with (v:=v) as [m']; eauto.
-    destruct* Hself as (co & loc_self & loc_struct & ofs & Hget_self & Hload_self & Hget_co & Hmem & ?).
-    exists m'; split*; constructor*.
-
-    - unfold compat_vars; intros x' t' ? Hin'.
-      edestruct Hvars as (loc' & Hget' & ? & Hm); eauto.
-      exists loc'; splits*.
-      + apply* Memory.Mem.store_valid_access_1.
-      + intros v' Hfind.
-        destruct (AST.ident_eq x' x).
-        *{ subst x'.
-           apply find_update_var in Hfind; subst v'.
-           specializes Hnodupvars Hin Hin'; subst t'. 
-           split*.
-           destruct (Values.eq_block loc' loc) as [|Neq].
-           - subst loc'.
-             rewrite Hloadres; apply* Memory.Mem.load_store_same.
-           - rewrite Hget in Hget'; inverts Hget'. now contradict Neq. 
-         }
-        *{ apply gso_var in Hfind; auto.
-           forwards (Hload & ?): Hm Hfind. 
-           split*.
-           destruct (Values.eq_block loc' loc).
-           - subst loc'.
-             edestruct Hnodupenv; eauto. 
-           - rewrite <-Hload. 
-             apply* Memory.Mem.load_store_other.
-         }        
-         
-    - unfold compat_self; intro.
-      exists co loc_self loc_struct ofs.
-      splits*.
-      + destruct (Values.eq_block loc_self loc).
-        * subst loc.
-          edestruct Hnodupenv; eauto.
-        * rewrite <-Hload_self.
-          apply* Memory.Mem.load_store_other.
-      + intros x' t' Hin'.
-        specializes Hmem Hin'; destruct Hmem as (delta & ? & ? & ? & Hm).
-        exists delta; splits*.
-         * apply* Memory.Mem.store_valid_access_1.
-         *{ intros v' Hfind.
-            apply find_field_update_var in Hfind.
-            forwards (Hload & ?): Hm Hfind.
-            splits*.
-            destruct (Values.eq_block loc loc_struct).
-            - edestruct Hsep; eauto.
-            - rewrite <-Hload.
-              apply* Memory.Mem.load_store_other.
-          }
-
-    - unfold mem_sep; introv ? ? Hget_self' ?.
-      rewrite Hget_self' in Hget_self; inverts Hget_self.
-      forwards* Eq: load_same; inverts Eq.
-      apply* Hsep.
-
-    - unfold self_sep; introv Hget_self' ?.
-      rewrite Hget_self' in Hget_self; inverts Hget_self.
-      forwards* Eq: load_same; inverts Eq.
-      apply* Hself_sep.
-  Qed.
-
-  (* Lemma compat_assigns_pres: *)
-  (*   forall c S e m loc ys vs, *)
+  (* Lemma compat_assign_pres: *)
+  (*   forall c S e m loc x t v, *)
   (*     In c prog -> *)
   (*     match_states c S (e, m) -> *)
-  (*     Nelist.Forall (fun y => In y (class_vars c)) ys -> *)
+  (*     Maps.PTree.get x e = Some (loc, t) -> *)
+  (*     In (x, t) (class_vars c) -> *)
+  (*     v = Values.Val.load_result (chunk_of_type t) v -> *)
+  (*     valid_val v t -> *)
+  (*     x <> self_id -> *)
   (*     exists m', Memory.Mem.store (chunk_of_type t) m loc 0 v = Some m'  *)
   (*           /\ match_states c (update_var S x v) (e, m'). *)
   (* Proof. *)
@@ -622,433 +793,507 @@ Section PRESERVATION.
   (*     apply* Hself_sep. *)
   (* Qed. *)
 
-  Remark load_same':
-    forall c env m m' chk loc' v ofs loc1 ofs1 loc2 ofs2,
-      self_sep c env m ->
-      Maps.PTree.get self_id env = Some (loc', pointer_of_node c.(c_name)) ->
-      Memory.Mem.store chk m loc1 ofs v = Some m' ->
-      Memory.Mem.load AST.Mint32 m loc' 0 = Some (Values.Vptr loc1 ofs1) ->
-      Memory.Mem.load AST.Mint32 m' loc' 0 = Some (Values.Vptr loc2 ofs2) ->
-      Values.Vptr loc1 ofs1 = Values.Vptr loc2 ofs2.
-  Proof.
-    introv Hself_sep ? ? Hload1 Hload2.
-    assert (Memory.Mem.load AST.Mint32 m' loc' 0 = Memory.Mem.load AST.Mint32 m loc' 0)
-      as Eq.
-    apply* Memory.Mem.load_store_other.
-    left; intro Eq; symmetry in Eq; revert Eq; apply* Hself_sep.
-    rewrite Eq in Hload2; rewrite Hload2 in Hload1; inverts Hload1.
-    reflexivity.
-  Qed.
+  (* (* Lemma compat_assigns_pres: *) *)
+  (* (*   forall c S e m loc ys vs, *) *)
+  (* (*     In c prog -> *) *)
+  (* (*     match_states c S (e, m) -> *) *)
+  (* (*     Nelist.Forall (fun y => In y (class_vars c)) ys -> *) *)
+  (* (*     exists m', Memory.Mem.store (chunk_of_type t) m loc 0 v = Some m'  *) *)
+  (* (*           /\ match_states c (update_var S x v) (e, m'). *) *)
+  (* (* Proof. *) *)
+  (* (*   introv ? MS Hget Hin Hloadres ? ?. *) *)
+  (* (*   inverts MS as Hvars Hself Hstep Hsep Hself_sep Hfields_sep Hnodupenv Hnodupvars; intro Hnodupmems. *) *)
+  (* (*   edestruct Hvars as (loc' & Hget' & ? & ?); eauto. *) *)
+  (* (*   rewrite Hget' in Hget; inverts Hget; rename Hget' into Hget. *) *)
+  (* (*   edestruct Memory.Mem.valid_access_store with (v:=v) as [m']; eauto. *) *)
+  (* (*   destruct* Hself as (co & loc_self & loc_struct & ofs & Hget_self & Hload_self & Hget_co & Hmem & ?). *) *)
+  (* (*   exists m'; split*; constructor*. *) *)
 
-  Lemma compat_stassign_pres:
-    forall c S e m x t v co loc_self loc_struct ofs delta,
-      In c prog ->
-      match_states c S (e, m) ->
-      Ctypes.field_offset tge.(Clight.genv_cenv) x (Ctypes.co_members co) = Errors.OK delta ->
-      Maps.PTree.get c.(c_name) (Clight.genv_cenv tge) = Some co ->
-      Maps.PTree.get self_id e = Some (loc_self, pointer_of_node c.(c_name)) ->
-      Memory.Mem.load AST.Mint32 m loc_self 0 = Some (Values.Vptr loc_struct ofs) ->
-      In (x, t) c.(c_mems) ->
-      v = Values.Val.load_result (chunk_of_type t) v ->
-      valid_val v t ->
-     Memory.Mem.valid_access m (chunk_of_type t) loc_struct (Int.unsigned (Int.add ofs (Int.repr delta))) Memtype.Writable ->
-      exists m',
-        Memory.Mem.store (chunk_of_type t) m loc_struct (Int.unsigned (Int.add ofs (Int.repr delta))) v = Some m'
-        /\ match_states c (update_field S x v) (e, m').
-  Proof.
-    intros ** ? MS Hoffset Hget_co Hget_self Hload_self Hin Hloadres ? ? .
-    inverts MS as Hvars Hself Hstep Hsep Hself_sep Hfields_sep Hnodupenv Hnodupvars; intro Hnodupmems.
-    edestruct Memory.Mem.valid_access_store with (v:=v) as [m']; eauto. 
-    exists m'; split*; constructor*.
+  (* (*   - unfold compat_vars; intros x' t' ? Hin'. *) *)
+  (* (*     edestruct Hvars as (loc' & Hget' & ? & Hm); eauto. *) *)
+  (* (*     exists loc'; splits*. *) *)
+  (* (*     + apply* Memory.Mem.store_valid_access_1. *) *)
+  (* (*     + intros v' Hfind. *) *)
+  (* (*       destruct (AST.ident_eq x' x). *) *)
+  (* (*       *{ subst x'. *) *)
+  (* (*          apply find_update_var in Hfind; subst v'. *) *)
+  (* (*          specializes Hnodupvars Hin Hin'; subst t'.  *) *)
+  (* (*          split*. *) *)
+  (* (*          destruct (Values.eq_block loc' loc) as [|Neq]. *) *)
+  (* (*          - subst loc'. *) *)
+  (* (*            rewrite Hloadres; apply* Memory.Mem.load_store_same. *) *)
+  (* (*          - rewrite Hget in Hget'; inverts Hget'. now contradict Neq.  *) *)
+  (* (*        } *) *)
+  (* (*       *{ apply gso_var in Hfind; auto. *) *)
+  (* (*          forwards (Hload & ?): Hm Hfind.  *) *)
+  (* (*          split*. *) *)
+  (* (*          destruct (Values.eq_block loc' loc). *) *)
+  (* (*          - subst loc'. *) *)
+  (* (*            edestruct Hnodupenv; eauto.  *) *)
+  (* (*          - rewrite <-Hload.  *) *)
+  (* (*            apply* Memory.Mem.load_store_other. *) *)
+  (* (*        }         *) *)
+         
+  (* (*   - unfold compat_self; intro. *) *)
+  (* (*     exists co loc_self loc_struct ofs. *) *)
+  (* (*     splits*. *) *)
+  (* (*     + destruct (Values.eq_block loc_self loc). *) *)
+  (* (*       * subst loc. *) *)
+  (* (*         edestruct Hnodupenv; eauto. *) *)
+  (* (*       * rewrite <-Hload_self. *) *)
+  (* (*         apply* Memory.Mem.load_store_other. *) *)
+  (* (*     + intros x' t' Hin'. *) *)
+  (* (*       specializes Hmem Hin'; destruct Hmem as (delta & ? & ? & ? & Hm). *) *)
+  (* (*       exists delta; splits*. *) *)
+  (* (*        * apply* Memory.Mem.store_valid_access_1. *) *)
+  (* (*        *{ intros v' Hfind. *) *)
+  (* (*           apply find_field_update_var in Hfind. *) *)
+  (* (*           forwards (Hload & ?): Hm Hfind. *) *)
+  (* (*           splits*. *) *)
+  (* (*           destruct (Values.eq_block loc loc_struct). *) *)
+  (* (*           - edestruct Hsep; eauto. *) *)
+  (* (*           - rewrite <-Hload. *) *)
+  (* (*             apply* Memory.Mem.load_store_other. *) *)
+  (* (*         } *) *)
 
-    - unfold compat_vars; intros.
-      edestruct Hvars as (loc & ? & ? & Hm); eauto.
-      exists loc; splits*.
-      + apply* Memory.Mem.store_valid_access_1.
-      + introv Hfind.
-        apply find_var_update_field in Hfind.
-        forwards (Hload & ?): Hm Hfind.
-        split*.
-        destruct (Values.eq_block loc loc_struct).
-        * edestruct Hsep; eauto.
-        * rewrite <-Hload.
-          apply* Memory.Mem.load_store_other.
+  (* (*   - unfold mem_sep; introv ? ? Hget_self' ?. *) *)
+  (* (*     rewrite Hget_self' in Hget_self; inverts Hget_self. *) *)
+  (* (*     forwards* Eq: load_same; inverts Eq. *) *)
+  (* (*     apply* Hsep. *) *)
 
-    - unfold compat_self; intro.
-      exists co loc_self loc_struct ofs.
-      destruct* Hself as (? & ? & ? & ? & Hget_self' & Hload_self' & Hget_co' & Hmem & ?).
-      rewrite Hget_co' in Hget_co; inverts Hget_co.
-      rewrite Hget_self' in Hget_self; inverts Hget_self.
-      rewrite Hload_self' in Hload_self; inverts Hload_self.  
-      splits*.
-      + destruct (Values.eq_block loc_self loc_struct).
-        * edestruct Hself_sep; eauto.
-        * rewrite <-Hload_self'.
-          apply* Memory.Mem.load_store_other.
-      + intros x' t' Hin'.
-        specializes Hmem Hin'; destruct Hmem as (delta' & Hoffset' & ? & ? & Hm).
-        exists delta'; splits*.
-        * apply* Memory.Mem.store_valid_access_1.  
-        *{ intros v' Hfind'.
-           destruct (AST.ident_eq x' x).
-           - subst x'.
-             rewrite Hoffset' in Hoffset; inverts Hoffset.
-             apply find_update_field in Hfind'; subst v'.
-             specializes Hnodupmems Hin Hin'; subst t'. 
-             split*.
-             rewrite Hloadres; apply* Memory.Mem.load_store_same.
-           - apply gso_field in Hfind'; auto.
-             forwards (Hload & ?): Hm Hfind'.
-             split*.
-             rewrite <-Hload; apply* Memory.Mem.load_store_other.
-         }
+  (* (*   - unfold self_sep; introv Hget_self' ?. *) *)
+  (* (*     rewrite Hget_self' in Hget_self; inverts Hget_self. *) *)
+  (* (*     forwards* Eq: load_same; inverts Eq. *) *)
+  (* (*     apply* Hself_sep. *) *)
+  (* (* Qed. *) *)
+
+  (* Remark load_same': *)
+  (*   forall c env m m' chk loc' v ofs loc1 ofs1 loc2 ofs2, *)
+  (*     self_sep c env m -> *)
+  (*     Maps.PTree.get self_id env = Some (loc', pointer_of_node c.(c_name)) -> *)
+  (*     Memory.Mem.store chk m loc1 ofs v = Some m' -> *)
+  (*     Memory.Mem.load AST.Mint32 m loc' 0 = Some (Values.Vptr loc1 ofs1) -> *)
+  (*     Memory.Mem.load AST.Mint32 m' loc' 0 = Some (Values.Vptr loc2 ofs2) -> *)
+  (*     Values.Vptr loc1 ofs1 = Values.Vptr loc2 ofs2. *)
+  (* Proof. *)
+  (*   introv Hself_sep ? ? Hload1 Hload2. *)
+  (*   assert (Memory.Mem.load AST.Mint32 m' loc' 0 = Memory.Mem.load AST.Mint32 m loc' 0) *)
+  (*     as Eq. *)
+  (*   apply* Memory.Mem.load_store_other. *)
+  (*   left; intro Eq; symmetry in Eq; revert Eq; apply* Hself_sep. *)
+  (*   rewrite Eq in Hload2; rewrite Hload2 in Hload1; inverts Hload1. *)
+  (*   reflexivity. *)
+  (* Qed. *)
+
+  (* Lemma compat_stassign_pres: *)
+  (*   forall c S e m x t v co loc_self loc_struct ofs delta, *)
+  (*     In c prog -> *)
+  (*     match_states c S (e, m) -> *)
+  (*     Ctypes.field_offset tge.(Clight.genv_cenv) x (Ctypes.co_members co) = Errors.OK delta -> *)
+  (*     Maps.PTree.get c.(c_name) (Clight.genv_cenv tge) = Some co -> *)
+  (*     Maps.PTree.get self_id e = Some (loc_self, pointer_of_node c.(c_name)) -> *)
+  (*     Memory.Mem.load AST.Mint32 m loc_self 0 = Some (Values.Vptr loc_struct ofs) -> *)
+  (*     In (x, t) c.(c_mems) -> *)
+  (*     v = Values.Val.load_result (chunk_of_type t) v -> *)
+  (*     valid_val v t -> *)
+  (*    Memory.Mem.valid_access m (chunk_of_type t) loc_struct (Int.unsigned (Int.add ofs (Int.repr delta))) Memtype.Writable -> *)
+  (*     exists m', *)
+  (*       Memory.Mem.store (chunk_of_type t) m loc_struct (Int.unsigned (Int.add ofs (Int.repr delta))) v = Some m' *)
+  (*       /\ match_states c (update_field S x v) (e, m'). *)
+  (* Proof. *)
+  (*   intros ** ? MS Hoffset Hget_co Hget_self Hload_self Hin Hloadres ? ? . *)
+  (*   inverts MS as Hvars Hself Hstep Hsep Hself_sep Hfields_sep Hnodupenv Hnodupvars; intro Hnodupmems. *)
+  (*   edestruct Memory.Mem.valid_access_store with (v:=v) as [m']; eauto.  *)
+  (*   exists m'; split*; constructor*. *)
+
+  (*   - unfold compat_vars; intros. *)
+  (*     edestruct Hvars as (loc & ? & ? & Hm); eauto. *)
+  (*     exists loc; splits*. *)
+  (*     + apply* Memory.Mem.store_valid_access_1. *)
+  (*     + introv Hfind. *)
+  (*       apply find_var_update_field in Hfind. *)
+  (*       forwards (Hload & ?): Hm Hfind. *)
+  (*       split*. *)
+  (*       destruct (Values.eq_block loc loc_struct). *)
+  (*       * edestruct Hsep; eauto. *)
+  (*       * rewrite <-Hload. *)
+  (*         apply* Memory.Mem.load_store_other. *)
+
+  (*   - unfold compat_self; intro. *)
+  (*     exists co loc_self loc_struct ofs. *)
+  (*     destruct* Hself as (? & ? & ? & ? & Hget_self' & Hload_self' & Hget_co' & Hmem & ?). *)
+  (*     rewrite Hget_co' in Hget_co; inverts Hget_co. *)
+  (*     rewrite Hget_self' in Hget_self; inverts Hget_self. *)
+  (*     rewrite Hload_self' in Hload_self; inverts Hload_self.   *)
+  (*     splits*. *)
+  (*     + destruct (Values.eq_block loc_self loc_struct). *)
+  (*       * edestruct Hself_sep; eauto. *)
+  (*       * rewrite <-Hload_self'. *)
+  (*         apply* Memory.Mem.load_store_other. *)
+  (*     + intros x' t' Hin'. *)
+  (*       specializes Hmem Hin'; destruct Hmem as (delta' & Hoffset' & ? & ? & Hm). *)
+  (*       exists delta'; splits*. *)
+  (*       * apply* Memory.Mem.store_valid_access_1.   *)
+  (*       *{ intros v' Hfind'. *)
+  (*          destruct (AST.ident_eq x' x). *)
+  (*          - subst x'. *)
+  (*            rewrite Hoffset' in Hoffset; inverts Hoffset. *)
+  (*            apply find_update_field in Hfind'; subst v'. *)
+  (*            specializes Hnodupmems Hin Hin'; subst t'.  *)
+  (*            split*. *)
+  (*            rewrite Hloadres; apply* Memory.Mem.load_store_same. *)
+  (*          - apply gso_field in Hfind'; auto. *)
+  (*            forwards (Hload & ?): Hm Hfind'. *)
+  (*            split*. *)
+  (*            rewrite <-Hload; apply* Memory.Mem.load_store_other. *)
+  (*        } *)
         
-    - unfold mem_sep; introv ? ? Hget_self' ?.
-      rewrite Hget_self' in Hget_self; inverts Hget_self.
-      forwards* Eq: load_same'; inverts Eq.
-      apply* Hsep.
+  (*   - unfold mem_sep; introv ? ? Hget_self' ?. *)
+  (*     rewrite Hget_self' in Hget_self; inverts Hget_self. *)
+  (*     forwards* Eq: load_same'; inverts Eq. *)
+  (*     apply* Hsep. *)
 
-    - unfold self_sep; introv Hget_self' ?.
-      rewrite Hget_self' in Hget_self; inverts Hget_self.
-      forwards* Eq: load_same'; inverts Eq.
-      apply* Hself_sep.
-  Qed.
+  (*   - unfold self_sep; introv Hget_self' ?. *)
+  (*     rewrite Hget_self' in Hget_self; inverts Hget_self. *)
+  (*     forwards* Eq: load_same'; inverts Eq. *)
+  (*     apply* Hself_sep. *)
+  (* Qed. *)
   
-  Remark alloc_exists:
-    forall vars e m,
-      exists e' m',
-        Clight.alloc_variables tge e m vars e' m'.
-  Proof.
-    induction vars as [|(x, ty)].
-    - do 3 econstructor.
-    - intros.
-      destruct (Memory.Mem.alloc m 0 (Ctypes.sizeof (Clight.genv_cenv tge) ty)) eqn: Eq.
-      specialize (IHvars (Maps.PTree.set x (b, ty) e) m0).
-      destruct* IHvars as (? & ? & ?).
-      do 3 econstructor; eauto.
-  Qed.
+  (* Remark alloc_exists: *)
+  (*   forall vars e m, *)
+  (*     exists e' m', *)
+  (*       Clight.alloc_variables tge e m vars e' m'. *)
+  (* Proof. *)
+  (*   induction vars as [|(x, ty)]. *)
+  (*   - do 3 econstructor. *)
+  (*   - intros. *)
+  (*     destruct (Memory.Mem.alloc m 0 (Ctypes.sizeof (Clight.genv_cenv tge) ty)) eqn: Eq. *)
+  (*     specialize (IHvars (Maps.PTree.set x (b, ty) e) m0). *)
+  (*     destruct* IHvars as (? & ? & ?). *)
+  (*     do 3 econstructor; eauto. *)
+  (* Qed. *)
 
-  Remark assign_loc_exists:
-    forall v ty m loc,
-      Ctypes.access_mode ty = Ctypes.By_value (chunk_of_type ty) ->
-      Memory.Mem.valid_access m (chunk_of_type ty) loc 0 Memtype.Writable ->
-      exists m',
-        Clight.assign_loc tge.(Clight.genv_cenv) ty m loc Int.zero v m'.
-  Proof.
-    introv ? Hvalid.
-    forwards (? & ?): Memory.Mem.valid_access_store Hvalid.
-    do 2 econstructor; eauto.
-  Qed.
+  (* Remark assign_loc_exists: *)
+  (*   forall v ty m loc, *)
+  (*     Ctypes.access_mode ty = Ctypes.By_value (chunk_of_type ty) -> *)
+  (*     Memory.Mem.valid_access m (chunk_of_type ty) loc 0 Memtype.Writable -> *)
+  (*     exists m', *)
+  (*       Clight.assign_loc tge.(Clight.genv_cenv) ty m loc Int.zero v m'. *)
+  (* Proof. *)
+  (*   introv ? Hvalid. *)
+  (*   forwards (? & ?): Memory.Mem.valid_access_store Hvalid. *)
+  (*   do 2 econstructor; eauto. *)
+  (* Qed. *)
   
-  Remark bind_parameters_exists:
-    forall xs vs e m,
-      length xs = length vs ->
-      Forall (fun x => exists loc,
-                  Maps.PTree.get (fst x) e = Some (loc, snd x)
-                  /\ Memory.Mem.valid_access m (chunk_of_type (snd x)) loc 0 Memtype.Writable
-                  /\ Ctypes.access_mode (snd x) = Ctypes.By_value (chunk_of_type (snd x))) xs ->
-      exists m',
-        Clight.bind_parameters tge e m xs vs m'.
-  Proof.
-    induction xs as [|(x, ty)]; destruct vs; introv Hlengths Hparams; try discriminate.
-    - do 2 econstructor.
-    - inverts Hparams as (? & ? & Hvalid & Haccess) Hparams.  
-      forwards (m' & Hassign): (assign_loc_exists v) Haccess Hvalid.
-      edestruct IHxs with (m:=m') (e:=e); eauto.
-      + inversion_clear Hassign as [|? ? ? ? Haccess'].
-        *{ clear IHxs Hlengths. induction xs.
-           - constructor.
-           - inverts Hparams as (loc & ?).
-             constructor.
-             + exists loc; splits*.
-               apply* Memory.Mem.store_valid_access_1.
-             + apply* IHxs.
-         }
-        * rewrite Haccess' in Haccess; discriminate.
-      + do 2 econstructor; eauto. 
-  Qed.
+  (* Remark bind_parameters_exists: *)
+  (*   forall xs vs e m, *)
+  (*     length xs = length vs -> *)
+  (*     Forall (fun x => exists loc, *)
+  (*                 Maps.PTree.get (fst x) e = Some (loc, snd x) *)
+  (*                 /\ Memory.Mem.valid_access m (chunk_of_type (snd x)) loc 0 Memtype.Writable *)
+  (*                 /\ Ctypes.access_mode (snd x) = Ctypes.By_value (chunk_of_type (snd x))) xs -> *)
+  (*     exists m', *)
+  (*       Clight.bind_parameters tge e m xs vs m'. *)
+  (* Proof. *)
+  (*   induction xs as [|(x, ty)]; destruct vs; introv Hlengths Hparams; try discriminate. *)
+  (*   - do 2 econstructor. *)
+  (*   - inverts Hparams as (? & ? & Hvalid & Haccess) Hparams.   *)
+  (*     forwards (m' & Hassign): (assign_loc_exists v) Haccess Hvalid. *)
+  (*     edestruct IHxs with (m:=m') (e:=e); eauto. *)
+  (*     + inversion_clear Hassign as [|? ? ? ? Haccess']. *)
+  (*       *{ clear IHxs Hlengths. induction xs. *)
+  (*          - constructor. *)
+  (*          - inverts Hparams as (loc & ?). *)
+  (*            constructor. *)
+  (*            + exists loc; splits*. *)
+  (*              apply* Memory.Mem.store_valid_access_1. *)
+  (*            + apply* IHxs. *)
+  (*        } *)
+  (*       * rewrite Haccess' in Haccess; discriminate. *)
+  (*     + do 2 econstructor; eauto.  *)
+  (* Qed. *)
 
-  Remark alloc_variables_implies:
-    forall vars e m e' m', 
-      Clight.alloc_variables tge e m vars e' m' ->
-      Forall (fun x => Ctypes.access_mode (snd x) = Ctypes.By_value (chunk_of_type (snd x))) vars ->
-      Forall (fun x => exists loc,
-                  Maps.PTree.get (fst x) e' = Some (loc, snd x)
-                  /\ Memory.Mem.valid_access m' (chunk_of_type (snd x)) loc 0 Memtype.Writable
-                  /\ Ctypes.access_mode (snd x) = Ctypes.By_value (chunk_of_type (snd x))) vars.
-  Proof.
-    induction vars.
-    - constructor.
-    - introv Halloc Hforall.
-      inverts Halloc.
-      constructor.
-      + exists b1; splits*.
-        * admit.
-        *{ assert (Memory.Mem.valid_access m1 (chunk_of_type (snd (id, ty))) b1 0 Memtype.Writable).
-           - eapply Memory.Mem.valid_access_freeable_any.
-             apply* Memory.Mem.valid_access_alloc_same.
-             + omega.
-             + simpl. admit.
-             + eapply BinInt.Z.divide_0_r.
-           - admit.
-         }
-        * inverts* Hforall.
-      + apply* IHvars.
-        inverts* Hforall.
-  Qed.
+  (* Remark alloc_variables_implies: *)
+  (*   forall vars e m e' m',  *)
+  (*     Clight.alloc_variables tge e m vars e' m' -> *)
+  (*     Forall (fun x => Ctypes.access_mode (snd x) = Ctypes.By_value (chunk_of_type (snd x))) vars -> *)
+  (*     Forall (fun x => exists loc, *)
+  (*                 Maps.PTree.get (fst x) e' = Some (loc, snd x) *)
+  (*                 /\ Memory.Mem.valid_access m' (chunk_of_type (snd x)) loc 0 Memtype.Writable *)
+  (*                 /\ Ctypes.access_mode (snd x) = Ctypes.By_value (chunk_of_type (snd x))) vars. *)
+  (* Proof. *)
+  (*   induction vars. *)
+  (*   - constructor. *)
+  (*   - introv Halloc Hforall. *)
+  (*     inverts Halloc. *)
+  (*     constructor. *)
+  (*     + exists b1; splits*. *)
+  (*       * admit. *)
+  (*       *{ assert (Memory.Mem.valid_access m1 (chunk_of_type (snd (id, ty))) b1 0 Memtype.Writable). *)
+  (*          - eapply Memory.Mem.valid_access_freeable_any. *)
+  (*            apply* Memory.Mem.valid_access_alloc_same. *)
+  (*            + omega. *)
+  (*            + simpl. admit. *)
+  (*            + eapply BinInt.Z.divide_0_r. *)
+  (*          - admit. *)
+  (*        } *)
+  (*       * inverts* Hforall. *)
+  (*     + apply* IHvars. *)
+  (*       inverts* Hforall. *)
+  (* Qed. *)
 
-  Remark forall_app:
-    forall A (P: A -> Prop) l1 l2,
-      Forall P (l1 ++ l2) -> Forall P l1 /\ Forall P l2.
-  Proof.
-    introv HForall; split; rewrite Forall_forall in *; introv Hin;
-    apply HForall; apply in_or_app; [left | right]; auto.
-  Qed.
+  (* Remark forall_app: *)
+  (*   forall A (P: A -> Prop) l1 l2, *)
+  (*     Forall P (l1 ++ l2) -> Forall P l1 /\ Forall P l2. *)
+  (* Proof. *)
+  (*   introv HForall; split; rewrite Forall_forall in *; introv Hin; *)
+  (*   apply HForall; apply in_or_app; [left | right]; auto. *)
+  (* Qed. *)
 
-  Lemma compat_funcall_pres:
-    forall m f vargs,
-      Datatypes.length (Clight.fn_params f) = Datatypes.length vargs ->
-      Forall (fun x => Ctypes.access_mode (snd x) = Ctypes.By_value (chunk_of_type (snd x))) (f.(Clight.fn_params) ++ f.(Clight.fn_vars)) ->
-      exists m1 e_fun m2,
-        Clight.alloc_variables tge Clight.empty_env m (f.(Clight.fn_params) ++ f.(Clight.fn_vars)) e_fun m1 
-        /\ Clight.bind_parameters tge e_fun m1 f.(Clight.fn_params) vargs m2.
-  Proof.
-    introv Hlengths Haccesses.
-    forwards (e_fun & m1 & Halloc):
-      (alloc_exists (f.(Clight.fn_params) ++ f.(Clight.fn_vars)) Clight.empty_env m).
-    exists m1 e_fun.
-    forwards* Hforall': alloc_variables_implies Halloc Haccesses.
-    forwards (Hforall & H'): forall_app Hforall'; clear Hforall' H'.
-    forwards* (m2 & ?): bind_parameters_exists Hlengths Hforall.
-  Qed.
+  (* Lemma compat_funcall_pres: *)
+  (*   forall m f vargs, *)
+  (*     Datatypes.length (Clight.fn_params f) = Datatypes.length vargs -> *)
+  (*     Forall (fun x => Ctypes.access_mode (snd x) = Ctypes.By_value (chunk_of_type (snd x))) (f.(Clight.fn_params) ++ f.(Clight.fn_vars)) -> *)
+  (*     exists m1 e_fun m2, *)
+  (*       Clight.alloc_variables tge Clight.empty_env m (f.(Clight.fn_params) ++ f.(Clight.fn_vars)) e_fun m1  *)
+  (*       /\ Clight.bind_parameters tge e_fun m1 f.(Clight.fn_params) vargs m2. *)
+  (* Proof. *)
+  (*   introv Hlengths Haccesses. *)
+  (*   forwards (e_fun & m1 & Halloc): *)
+  (*     (alloc_exists (f.(Clight.fn_params) ++ f.(Clight.fn_vars)) Clight.empty_env m). *)
+  (*   exists m1 e_fun. *)
+  (*   forwards* Hforall': alloc_variables_implies Halloc Haccesses. *)
+  (*   forwards (Hforall & H'): forall_app Hforall'; clear Hforall' H'. *)
+  (*   forwards* (m2 & ?): bind_parameters_exists Hlengths Hforall. *)
+  (* Qed. *)
   
-  Remark type_pres':
-    forall c' c es ys,
-      Nelist.Forall2 (fun e x => typeof e = snd x) es c'.(c_input) ->
-      map Clight.typeof (nelist2list (Nelist.map (translate_exp c.(c_name)) es)
-                         ++ nelist2list (Nelist.map make_out_arg ys)) =
-      map snd (nelist2list c'.(c_input) ++ nelist2list c'.(c_output)).
-  Proof.
-    (* intros c'. *)
-    (* induction (c_input c'); introv Heq; *)
-    (* inversion_clear Heq as [? ? Hty|? ? ? ? Hty Hforall2]; simpl. *)
-    (* - rewrite type_pres, Hty; auto. *)
-    (* - f_equal. *)
-    (*   + rewrite type_pres, Hty; auto. *)
-    (*   + specializes IHn Hforall2; eauto. *)
-    admit.
-  Qed.
+  (* Remark type_pres': *)
+  (*   forall c' c es ys, *)
+  (*     Nelist.Forall2 (fun e x => typeof e = snd x) es c'.(c_input) -> *)
+  (*     map Clight.typeof (nelist2list (Nelist.map (translate_exp c.(c_name)) es) *)
+  (*                        ++ nelist2list (Nelist.map make_out_arg ys)) = *)
+  (*     map snd (nelist2list c'.(c_input) ++ nelist2list c'.(c_output)). *)
+  (* Proof. *)
+  (*   (* intros c'. *) *)
+  (*   (* induction (c_input c'); introv Heq; *) *)
+  (*   (* inversion_clear Heq as [? ? Hty|? ? ? ? Hty Hforall2]; simpl. *) *)
+  (*   (* - rewrite type_pres, Hty; auto. *) *)
+  (*   (* - f_equal. *) *)
+  (*   (*   + rewrite type_pres, Hty; auto. *) *)
+  (*   (*   + specializes IHn Hforall2; eauto. *) *)
+  (*   admit. *)
+  (* Qed. *)
 
-  Hint Constructors Clight.eval_lvalue Clight.eval_expr well_formed_stmt.
-  Hint Resolve expr_eval_simu Clight.assign_loc_value sem_cast_same.
-  Hint Constructors well_formed_stmt.
+  (* Hint Constructors Clight.eval_lvalue Clight.eval_expr well_formed_stmt. *)
+  (* Hint Resolve expr_eval_simu Clight.assign_loc_value sem_cast_same. *)
+  (* Hint Constructors well_formed_stmt. *)
 
-  Remark ne_Forall2_lengths:
-    forall A B (P: A -> B -> Prop) l1 l2,
-      Nelist.Forall2 P l1 l2 -> Nelist.length l1 = Nelist.length l2.
-  Proof.
-    induction l1, l2; introv HForall2; inverts* HForall2.
-    simpl; f_equal; apply* IHl1.
-  Qed.
+  (* Remark ne_Forall2_lengths: *)
+  (*   forall A B (P: A -> B -> Prop) l1 l2, *)
+  (*     Nelist.Forall2 P l1 l2 -> Nelist.length l1 = Nelist.length l2. *)
+  (* Proof. *)
+  (*   induction l1, l2; introv HForall2; inverts* HForall2. *)
+  (*   simpl; f_equal; apply* IHl1. *)
+  (* Qed. *)
 
-  Lemma exprlist_make_out_arg:
-    forall c S e le m ys,
-      In c prog ->
-      compat_vars c S e m ->
-      Nelist.Forall (fun y => In y (class_vars c)) ys ->
-      exists vs, Clight.eval_exprlist tge e le m
-                                 (nelist2list (Nelist.map make_out_arg ys))
-                                 (list_type_to_typelist
-                                    (map Clight.typeof (nelist2list (Nelist.map make_out_arg ys))))
-                                 vs.
-  Proof.
-    introv ? Hvars Hins.
-    induction ys as [[x t]|[x t]]; inverts Hins as ? Hins;
-    edestruct Hvars; eauto.
-    - do 2 econstructor; eauto.
-      + apply Clight.eval_Eaddrof.
-        apply* Clight.eval_Evar_local.
-      + apply sem_cast_same.
-        simpl. splits*.
-        * discriminate.
-        * unfold pointer_of; simpl; trivial.
-    - forwards (? & ?): IHys Hins.
-      simpl.
-      do 2 econstructor; eauto.
-      + apply Clight.eval_Eaddrof.
-        apply* Clight.eval_Evar_local.
-      + apply sem_cast_same.
-        splits*.
-        * discriminate.
-        * unfold pointer_of; simpl; trivial.
-  Qed.
+  (* Lemma exprlist_make_out_arg: *)
+  (*   forall c S e le m ys, *)
+  (*     In c prog -> *)
+  (*     compat_vars c S e m -> *)
+  (*     Nelist.Forall (fun y => In y (class_vars c)) ys -> *)
+  (*     exists vs, Clight.eval_exprlist tge e le m *)
+  (*                                (nelist2list (Nelist.map make_out_arg ys)) *)
+  (*                                (list_type_to_typelist *)
+  (*                                   (map Clight.typeof (nelist2list (Nelist.map make_out_arg ys)))) *)
+  (*                                vs. *)
+  (* Proof. *)
+  (*   introv ? Hvars Hins. *)
+  (*   induction ys as [[x t]|[x t]]; inverts Hins as ? Hins; *)
+  (*   edestruct Hvars; eauto. *)
+  (*   - do 2 econstructor; eauto. *)
+  (*     + apply Clight.eval_Eaddrof. *)
+  (*       apply* Clight.eval_Evar_local. *)
+  (*     + apply sem_cast_same. *)
+  (*       simpl. splits*. *)
+  (*       * discriminate. *)
+  (*       * unfold pointer_of; simpl; trivial. *)
+  (*   - forwards (? & ?): IHys Hins. *)
+  (*     simpl. *)
+  (*     do 2 econstructor; eauto. *)
+  (*     + apply Clight.eval_Eaddrof. *)
+  (*       apply* Clight.eval_Evar_local. *)
+  (*     + apply sem_cast_same. *)
+  (*       splits*. *)
+  (*       * discriminate. *)
+  (*       * unfold pointer_of; simpl; trivial. *)
+  (* Qed. *)
   
-  Theorem simu_bigbig:
-    (forall p S1 s S2,
-        stmt_eval p S1 s S2 ->
-        sub_prog p prog ->
-         forall c,
-          In c prog ->
-          forall e1 le1 m1
-            (WF: well_formed_stmt c S1 s) 
-            (MS: match_states c S1 (e1, m1)),
-          exists le2 m2 t,
-            exec_stmt tge (Clight.function_entry1 tge) e1 le1 m1
-                      (translate_stmt c.(c_name) s) t le2 m2 ClightBigstep.Out_normal
-            /\ match_states c S2 (e1, m2))
-    /\ (forall p me clsid vs me' rvs,
-          stmt_step_eval p me clsid vs me' rvs ->
-          sub_prog p prog ->
-          forall c S o c' prog' m loc_f f loc_struct ofs e le outs,
-            In c' prog ->
-            well_formed_stmt c' (me, adds (Nelist.map_fst c'.(c_input)) vs v_empty) c'.(c_step) ->
-            match_states c S (e, m) ->
-            Globalenvs.Genv.find_symbol tge.(Clight.genv_genv) (step_id clsid) = Some loc_f ->
-            Globalenvs.Genv.find_funct_ptr tge.(Clight.genv_genv) loc_f = Some (Ctypes.Internal f) ->
-            find_inst S o me ->
-            find_class clsid prog = Some (c', prog') ->
-            List.length f.(Clight.fn_params) = 1 + Nelist.length vs + Nelist.length c'.(c_output) ->
-            Clight.eval_expr tge e le m (ptr_obj (Some c.(c_name)) clsid o) (Values.Vptr loc_struct ofs) ->
-            exists m' t,
-              eval_funcall tge (Clight.function_entry1 tge) m (Ctypes.Internal f)
-                           ((Values.Vptr loc_struct ofs) :: nelist2list vs ++ outs) t m' Values.Vundef
-              /\ match_states c (update_inst S o me') (e, m')
-        ).
-  Proof.
-    clear TRANSL.
-    apply stmt_eval_step_ind;
-      [| |introv ? ? ? ? Hifte|introv ? HS1 ? HS2|introv ? Evs ? Hrec_eval|
-       |(introv Hfind ? ? Hrec_exec; intros ** MS Hget_loc_f Hget_f ? Hfind' Hlengths ?)];
-      intros;
-      try inverts WF as; [|introv Hin| | |introv Hlengths' Hins Hin Hfind Wfs ? Valids Types| |]; intros;
-      inverts MS as Hvars Hself Hstep.
+  (* Theorem simu_bigbig: *)
+  (*   (forall p S1 s S2, *)
+  (*       stmt_eval p S1 s S2 -> *)
+  (*       sub_prog p prog -> *)
+  (*        forall c, *)
+  (*         In c prog -> *)
+  (*         forall e1 le1 m1 *)
+  (*           (WF: well_formed_stmt c S1 s)  *)
+  (*           (MS: match_states c S1 (e1, m1)), *)
+  (*         exists le2 m2 t, *)
+  (*           exec_stmt tge (Clight.function_entry1 tge) e1 le1 m1 *)
+  (*                     (translate_stmt c.(c_name) s) t le2 m2 ClightBigstep.Out_normal *)
+  (*           /\ match_states c S2 (e1, m2)) *)
+  (*   /\ (forall p me clsid vs me' rvs, *)
+  (*         stmt_step_eval p me clsid vs me' rvs -> *)
+  (*         sub_prog p prog -> *)
+  (*         forall c S o c' prog' m loc_f f loc_struct ofs e le outs, *)
+  (*           In c' prog -> *)
+  (*           well_formed_stmt c' (me, adds (Nelist.map_fst c'.(c_input)) vs v_empty) c'.(c_step) -> *)
+  (*           match_states c S (e, m) -> *)
+  (*           Globalenvs.Genv.find_symbol tge.(Clight.genv_genv) (step_id clsid) = Some loc_f -> *)
+  (*           Globalenvs.Genv.find_funct_ptr tge.(Clight.genv_genv) loc_f = Some (Ctypes.Internal f) -> *)
+  (*           find_inst S o me -> *)
+  (*           find_class clsid prog = Some (c', prog') -> *)
+  (*           List.length f.(Clight.fn_params) = 1 + Nelist.length vs + Nelist.length c'.(c_output) -> *)
+  (*           Clight.eval_expr tge e le m (ptr_obj (Some c.(c_name)) clsid o) (Values.Vptr loc_struct ofs) -> *)
+  (*           exists m' t, *)
+  (*             eval_funcall tge (Clight.function_entry1 tge) m (Ctypes.Internal f) *)
+  (*                          ((Values.Vptr loc_struct ofs) :: nelist2list vs ++ outs) t m' Values.Vundef *)
+  (*             /\ match_states c (update_inst S o me') (e, m') *)
+  (*       ). *)
+  (* Proof. *)
+  (*   clear TRANSL. *)
+  (*   apply stmt_eval_step_ind; *)
+  (*     [| |introv ? ? ? ? Hifte|introv ? HS1 ? HS2|introv ? Evs ? Hrec_eval| *)
+  (*      |(introv Hfind ? ? Hrec_exec; intros ** MS Hget_loc_f Hget_f ? Hfind' Hlengths ?)]; *)
+  (*     intros; *)
+  (*     try inverts WF as; [|introv Hin| | |introv Hlengths' Hins Hin Hfind Wfs ? Valids Types| |]; intros; *)
+  (*     inverts MS as Hvars Hself Hstep. *)
 
-    (* Assign x e : "x = e" *)
-    - app_exp_eval_det.
-      edestruct Hvars; eauto.
-      edestruct compat_assign_pres; iauto.  
-      do 3 econstructor; split*.
-      apply* ClightBigstep.exec_Sassign. 
-      rewrite* type_pres.
+  (*   (* Assign x e : "x = e" *) *)
+  (*   - app_exp_eval_det. *)
+  (*     edestruct Hvars; eauto. *)
+  (*     edestruct compat_assign_pres; iauto.   *)
+  (*     do 3 econstructor; split*. *)
+  (*     apply* ClightBigstep.exec_Sassign.  *)
+  (*     rewrite* type_pres. *)
 
-    (* AssignSt x e : "self->x = e"*)
-    - app_exp_eval_det.
-      pose proof Hself as Hself'.
-      destruct* Hself' as (? & ? & ? & ? & ? & ? & ? & Hmem & ?).
-      specializes Hmem Hin; destruct_conjs.    
-      edestruct compat_stassign_pres; iauto.      
-      do 3 econstructor; split*.
-      apply* ClightBigstep.exec_Sassign.
-      + apply* evall_self_field. 
-      + rewrite* type_pres.
+  (*   (* AssignSt x e : "self->x = e"*) *)
+  (*   - app_exp_eval_det. *)
+  (*     pose proof Hself as Hself'. *)
+  (*     destruct* Hself' as (? & ? & ? & ? & ? & ? & ? & Hmem & ?). *)
+  (*     specializes Hmem Hin; destruct_conjs.     *)
+  (*     edestruct compat_stassign_pres; iauto.       *)
+  (*     do 3 econstructor; split*. *)
+  (*     apply* ClightBigstep.exec_Sassign. *)
+  (*     + apply* evall_self_field.  *)
+  (*     + rewrite* type_pres. *)
         
-    (* Ifte e s1 s2 : "if e then s1 else s2" *)
-    - edestruct Hifte with (le1:=le1); destruct_conjs; eauto; [destruct* b|]. 
-      do 3 econstructor; split*.
-      apply* exec_Sifthenelse. 
-      + erewrite type_pres, bool_val_ptr; eauto.
-      + destruct* b. 
+  (*   (* Ifte e s1 s2 : "if e then s1 else s2" *) *)
+  (*   - edestruct Hifte with (le1:=le1); destruct_conjs; eauto; [destruct* b|].  *)
+  (*     do 3 econstructor; split*. *)
+  (*     apply* exec_Sifthenelse.  *)
+  (*     + erewrite type_pres, bool_val_ptr; eauto. *)
+  (*     + destruct* b.  *)
       
-    (* Comp s1 s2 : "s1; s2" *)
-    - app_stmt_eval_det'.
-      edestruct HS1; destruct_conjs; eauto.
-      edestruct HS2; destruct_conjs; eauto.
-      do 3 econstructor; split*.
-      apply* exec_Sseq_1.
+  (*   (* Comp s1 s2 : "s1; s2" *) *)
+  (*   - app_stmt_eval_det'. *)
+  (*     edestruct HS1; destruct_conjs; eauto. *)
+  (*     edestruct HS2; destruct_conjs; eauto. *)
+  (*     do 3 econstructor; split*. *)
+  (*     apply* exec_Sseq_1. *)
 
-    (* Step_ap y ty clsid o [e1; ... ;en] : "y = clsid_step(&(self->o), e1, ..., en)" *)
-    - app_exps_eval_det.
-      app_find_inst_det.
-      app_stmt_step_eval_det'.
+  (*   (* Step_ap y ty clsid o [e1; ... ;en] : "y = clsid_step(&(self->o), e1, ..., en)" *) *)
+  (*   - app_exps_eval_det. *)
+  (*     app_find_inst_det. *)
+  (*     app_stmt_step_eval_det'. *)
       
-      (* get the Clight corresponding function *)
-      forwards* Hin': find_class_In Hfind.
-      pose proof Hstep as Hstep'.
-      edestruct Hstep' as (loc_f & f & ? & ? & ? & Htype_fun & ? & ? & Hlengths & ?); eauto.
-      rewrite <-type_pres' with (c:=c) (es:=es) (ys:=ys) in Htype_fun; auto.
-      forwards Eq: find_class_name Hfind.
-      rewrite Eq in *; clear Eq.
+  (*     (* get the Clight corresponding function *) *)
+  (*     forwards* Hin': find_class_In Hfind. *)
+  (*     pose proof Hstep as Hstep'. *)
+  (*     edestruct Hstep' as (loc_f & f & ? & ? & ? & Htype_fun & ? & ? & Hlengths & ?); eauto. *)
+  (*     rewrite <-type_pres' with (c:=c) (es:=es) (ys:=ys) in Htype_fun; auto. *)
+  (*     forwards Eq: find_class_name Hfind. *)
+  (*     rewrite Eq in *; clear Eq. *)
       
-      (* get the Clight corresponding field *)
-      pose proof Hself as Hself'.
-      destruct* Hself' as (? & ? & ? & ? & ? & ? & ? & ? & Hobj).
-      specializes Hobj Hin; destruct Hobj. 
+  (*     (* get the Clight corresponding field *) *)
+  (*     pose proof Hself as Hself'. *)
+  (*     destruct* Hself' as (? & ? & ? & ? & ? & ? & ? & ? & Hobj). *)
+  (*     specializes Hobj Hin; destruct Hobj.  *)
 
-      (* get outs values *)
-      edestruct exprlist_make_out_arg with (le:=le1) (c:=c) as (outs); eauto.
+  (*     (* get outs values *) *)
+  (*     edestruct exprlist_make_out_arg with (le:=le1) (c:=c) as (outs); eauto. *)
       
-      (* recursive funcall evaluation *)
-      edestruct Hrec_eval with (c:=c) (e:=e1) (m:=m1) (le:=le1) (outs:=outs); destruct_conjs; eauto.
-      + rewrite <-ne_Forall2_lengths with (1:=Evs).
-        rewrite Hlengths; simpl; f_equal.
-        rewrite app_length; do 2 rewrite <-nelist2list_length.
-        f_equal; symmetry; apply* ne_Forall2_lengths.        
-      + apply Clight.eval_Eaddrof; apply* evall_self_field.
-      + do 3 econstructor; split*.
-        *{ apply* exec_Scall.
-           - simpl; eauto.
-           - eapply Clight.eval_Elvalue.
-             + apply* Clight.eval_Evar_global.
-             + apply* Clight.deref_loc_reference.
-           - econstructor.
-             + eapply Clight.eval_Eaddrof.
-               apply* evall_self_field.
-             + eapply sem_cast_same.
-               unfold valid_val; splits*.
-               * discriminate.
-               * simpl; trivial.
-             + apply* eval_exprlist_app.
-               apply* exprs_eval_simu.
-           - eauto.
-         }
-        * admit. 
+  (*     (* recursive funcall evaluation *) *)
+  (*     edestruct Hrec_eval with (c:=c) (e:=e1) (m:=m1) (le:=le1) (outs:=outs); destruct_conjs; eauto. *)
+  (*     + rewrite <-ne_Forall2_lengths with (1:=Evs). *)
+  (*       rewrite Hlengths; simpl; f_equal. *)
+  (*       rewrite app_length; do 2 rewrite <-nelist2list_length. *)
+  (*       f_equal; symmetry; apply* ne_Forall2_lengths.         *)
+  (*     + apply Clight.eval_Eaddrof; apply* evall_self_field. *)
+  (*     + do 3 econstructor; split*. *)
+  (*       *{ apply* exec_Scall. *)
+  (*          - simpl; eauto. *)
+  (*          - eapply Clight.eval_Elvalue. *)
+  (*            + apply* Clight.eval_Evar_global. *)
+  (*            + apply* Clight.deref_loc_reference. *)
+  (*          - econstructor. *)
+  (*            + eapply Clight.eval_Eaddrof. *)
+  (*              apply* evall_self_field. *)
+  (*            + eapply sem_cast_same. *)
+  (*              unfold valid_val; splits*. *)
+  (*              * discriminate. *)
+  (*              * simpl; trivial. *)
+  (*            + apply* eval_exprlist_app. *)
+  (*              apply* exprs_eval_simu. *)
+  (*          - eauto. *)
+  (*        } *)
+  (*       * admit.  *)
 
-    (* Skip : "skip" *)
-    - do 3 econstructor; split*.
-      eapply exec_Sskip.
+  (*   (* Skip : "skip" *) *)
+  (*   - do 3 econstructor; split*. *)
+  (*     eapply exec_Sskip. *)
 
-    (* funcall *)
-    - forwards* Hfind'': find_class_sub_same Hfind UNIQUE.
-      rewrite Hfind' in Hfind''; inverts Hfind''.
-      destruct Hstep with (c:=cls)
-        as (loc_f' & f' & Hget_loc_f' & Hget_f' & Htype_fun & Hvars_nil & ? & ? & Htr & ?);
-        destruct_conjs; eauto.
-      forwards Eq: find_class_name Hfind.
-      rewrite Eq in Hget_loc_f'; clear Eq.
-      rewrite Hget_loc_f' in Hget_loc_f; inverts Hget_loc_f.
-      rewrite Hget_f' in Hget_f; inverts Hget_f.
+  (*   (* funcall *) *)
+  (*   - forwards* Hfind'': find_class_sub_same Hfind UNIQUE. *)
+  (*     rewrite Hfind' in Hfind''; inverts Hfind''. *)
+  (*     destruct Hstep with (c:=cls) *)
+  (*       as (loc_f' & f' & Hget_loc_f' & Hget_f' & Htype_fun & Hvars_nil & ? & ? & Htr & ?); *)
+  (*       destruct_conjs; eauto. *)
+  (*     forwards Eq: find_class_name Hfind. *)
+  (*     rewrite Eq in Hget_loc_f'; clear Eq. *)
+  (*     rewrite Hget_loc_f' in Hget_loc_f; inverts Hget_loc_f. *)
+  (*     rewrite Hget_f' in Hget_f; inverts Hget_f. *)
 
-      assert (length f.(Clight.fn_params) = length ((Values.Vptr loc_struct ofs) :: nelist2list vs))
-        by (rewrite Hlengths; simpl; f_equal; rewrite Nelist.nelist2list_length; auto).
+  (*     assert (length f.(Clight.fn_params) = length ((Values.Vptr loc_struct ofs) :: nelist2list vs)) *)
+  (*       by (rewrite Hlengths; simpl; f_equal; rewrite Nelist.nelist2list_length; auto). *)
 
-      forwards* (le_fun & ? & ?): (compat_funcall_pres cls m).
-      forwards* Hsub: find_class_sub.
-      subst env.
-      edestruct Hrec_exec with (le1:=le_fun) as (? & ? & ? & ? & MS); eauto.
-      destruct_conjs.
+  (*     forwards* (le_fun & ? & ?): (compat_funcall_pres cls m). *)
+  (*     forwards* Hsub: find_class_sub. *)
+  (*     subst env. *)
+  (*     edestruct Hrec_exec with (le1:=le_fun) as (? & ? & ? & ? & MS); eauto. *)
+  (*     destruct_conjs. *)
         
-      do 2 econstructor; split.
-      apply* eval_funcall_internal.
-      + constructor*; rewrite Hvars_nil; simpl; constructor.
-      + rewrite* Htr.
-        apply* exec_Sseq_1.
-        apply* exec_Sreturn_some.
-        apply* Clight.eval_Etempvar.
-        inverts MS as Hvars'.
-        apply* Hvars'; rewrite <-surjective_pairing; eapply in_eq.
-      + simpl; split*.
-        inverts Htype_fun.
-        apply* sem_cast_same.
-      + simpl; eauto.       
-      + constructor*.
-        unfold compat_self.
-        intro Hin.
-        pose proof Hself as Hself'.
-        destruct* Hself' as (? & loc_struct' & ofs' & Hget_self' & Hget_co' & Hmem & Hobj).
-        do 3 econstructor; splits*.
-        intros x' t' Hin'. 
-        specializes Hmem Hin'; destruct Hmem.
-        econstructor; splits*.
-        * admit.
-        * admit.
-  Qed.
+  (*     do 2 econstructor; split. *)
+  (*     apply* eval_funcall_internal. *)
+  (*     + constructor*; rewrite Hvars_nil; simpl; constructor. *)
+  (*     + rewrite* Htr. *)
+  (*       apply* exec_Sseq_1. *)
+  (*       apply* exec_Sreturn_some. *)
+  (*       apply* Clight.eval_Etempvar. *)
+  (*       inverts MS as Hvars'. *)
+  (*       apply* Hvars'; rewrite <-surjective_pairing; eapply in_eq. *)
+  (*     + simpl; split*. *)
+  (*       inverts Htype_fun. *)
+  (*       apply* sem_cast_same. *)
+  (*     + simpl; eauto.        *)
+  (*     + constructor*. *)
+  (*       unfold compat_self. *)
+  (*       intro Hin. *)
+  (*       pose proof Hself as Hself'. *)
+  (*       destruct* Hself' as (? & loc_struct' & ofs' & Hget_self' & Hget_co' & Hmem & Hobj). *)
+  (*       do 3 econstructor; splits*. *)
+  (*       intros x' t' Hin'.  *)
+  (*       specializes Hmem Hin'; destruct Hmem. *)
+  (*       econstructor; splits*. *)
+  (*       * admit. *)
+  (*       * admit. *)
+  (* Qed. *)
